src/RGA.thy
@@ -1,6 +1,7 @@
 (* Victor B. F. Gomes, University of Cambridge
    Martin Kleppmann, University of Cambridge
    Dominic P. Mulligan, University of Cambridge
+   Alastair R. Beresford, University of Cambridge
 *)
 
 subsection\<open>Network\<close>
@@ -23,15 +24,15 @@ fun interpret_opers :: "('id::linorder, 'v) operation \<Rightarrow> ('id, 'v) el
 definition element_ids :: "('id, 'v) elt list \<Rightarrow> 'id set" where
  "element_ids list \<equiv> set (map fst list)"
 
-definition valid_rga_msgs :: "nat \<Rightarrow> ('id, 'v) elt list \<Rightarrow> ('id \<times> ('id::linorder, 'v) operation) set" where
- "valid_rga_msgs node list \<equiv> { (i::'id, oper::('id, 'v) operation). case oper of
-    Insert e  None      \<Rightarrow> fst e = i |
-    Insert e (Some pos) \<Rightarrow> fst e = i \<and> pos \<in> element_ids list |
-    Delete         pos  \<Rightarrow> pos \<in> element_ids list }"
- 
-(* Replicated Growable Array Network *)
-locale rga = network_with_constrained_ops _ interpret_opers "[]" valid_rga_msgs
+definition valid_rga_msg :: "('id, 'v) elt list \<Rightarrow> 'id \<times> ('id::linorder, 'v) operation \<Rightarrow> bool" where
+ "valid_rga_msg list msg \<equiv> case msg of
+    (i, Insert e  None     ) \<Rightarrow> fst e = i |
+    (i, Insert e (Some pos)) \<Rightarrow> fst e = i \<and> pos \<in> element_ids list |
+    (i, Delete         pos ) \<Rightarrow> pos \<in> element_ids list"
 
+(* Replicated Growable Array Network *)
+locale rga = network_with_constrained_ops _ interpret_opers "[]" valid_rga_msg
+  
 definition indices :: "('id \<times> ('id, 'v) operation) event list \<Rightarrow> 'id list" where
   "indices xs \<equiv>
      List.map_filter (\<lambda>x. case x of Deliver (i, Insert e n) \<Rightarrow> Some (fst e) | _ \<Rightarrow> None) xs"
@@ -66,19 +67,18 @@ lemma (in rga) apply_opers_idx_elems:
       and "apply_operations es = Some xs"
     shows "element_ids xs = set (indices es)"
 using assms unfolding element_ids_def
-  apply(induction es arbitrary: xs rule: rev_induct; clarsimp)
-  apply(case_tac x; clarsimp)
-  apply blast
-  apply(case_tac "b"; clarsimp)
-  apply(auto split: bind_splits simp add: interp_msg_def)
-  apply(metis (no_types, hide_lams) Un_insert_right image_eqI insert_iff insert_preserve_indices
-        option.sel prefix_of_appendD prod.sel(1) sup_bot.comm_neutral)
-  apply(metis Un_insert_right fst_conv insert_iff insert_preserve_indices option.sel)
-  apply(metis (no_types, hide_lams) Un_insert_right insert_iff insert_preserve_indices' option.sel
-        prefix_of_appendD sup_bot.comm_neutral)
-  apply(metis delete_preserve_indices fst_conv image_eqI prefix_of_appendD)
-  using delete_preserve_indices apply blast
-done
+proof(induction es arbitrary: xs rule: rev_induct, clarsimp)
+  case (snoc x xs) thus ?case
+  proof (cases x, clarsimp, blast)
+    case (Deliver e)
+    moreover obtain a b where "e = (a, b)" by force
+    ultimately show ?thesis
+      using snoc assms apply (cases b; clarsimp split: bind_splits simp add: interp_msg_def)
+       apply (metis Un_insert_right append.right_neutral insert_preserve_indices' list.set(1)
+              option.sel prefix_of_appendD prod.sel(1) set_append)
+      by (metis delete_preserve_indices prefix_of_appendD)
+  qed
+qed
 
 lemma (in rga) delete_does_not_change_element_ids:
   assumes "es @ [Deliver (i, Delete n)] prefix of j"
@@ -107,22 +107,33 @@ lemma (in rga) deliver_insert_exists:
       and "a \<in> element_ids xs"
     shows "\<exists>i v f n. Deliver (i, Insert (a, v, f) n) \<in> set es"
 using assms unfolding element_ids_def
-  apply(induction es arbitrary: xs rule: rev_induct; clarsimp)
-  apply(case_tac x; clarsimp)
-  apply(metis image_eqI prefix_of_appendD prod.sel(1))
-  apply(case_tac "bb"; clarsimp)
-  defer
-  apply(drule prefix_of_appendD, clarsimp simp add: bind_eq_Some_conv interp_msg_def)
-  apply(metis delete_preserve_indices image_eqI prod.sel(1))
-  apply(case_tac "aba=a")
-  apply blast
-  apply(subgoal_tac "\<exists>xs'. apply_operations xsa = Some xs'")
-  defer
-  apply(meson bind_eq_Some_conv)
-  apply(erule exE)
-  apply(metis (no_types, lifting) someone_inserted_id apply_operations_Deliver element_ids_def
-    image_eqI prefix_of_appendD prod.sel(1) set_map)
-done
+proof(induction es arbitrary: xs rule: rev_induct, clarsimp)
+  case (snoc x xs ys) thus ?case
+  proof (cases x)
+    case (Broadcast e) thus ?thesis
+      using snoc by(clarsimp, metis image_eqI prefix_of_appendD prod.sel(1))
+  next
+    case (Deliver e)
+    moreover then obtain xs' where *: "apply_operations xs = Some xs'"
+        using snoc by fastforce
+    moreover obtain k v where **: "e = (k, v)" by force
+    ultimately show ?thesis
+      using assms snoc proof (cases v)
+      case (Insert el _) thus ?thesis
+        using snoc Deliver * **
+        apply (cases el; cases "fst el = a"; clarsimp)
+        apply (blast, metis (no_types, lifting) element_ids_def prefix_of_appendD set_map snoc.prems(2)
+                      snoc.prems(3) someone_inserted_id)
+        done
+      next
+      case (Delete _) thus ?thesis
+        using snoc Deliver ** apply clarsimp
+        apply(drule prefix_of_appendD, clarsimp simp add: bind_eq_Some_conv interp_msg_def)
+        apply(metis delete_preserve_indices image_eqI prod.sel(1))
+        done
+    qed    
+  qed
+qed
 
 lemma (in rga) insert_in_apply_set:
   assumes "es @ [Deliver (i, Insert e (Some a))] prefix of j"
@@ -130,63 +141,54 @@ lemma (in rga) insert_in_apply_set:
       and "apply_operations es = Some s"
     shows "fst e' \<in> element_ids s"
 using assms apply_opers_idx_elems idx_in_elem_inserted prefix_of_appendD by blast
-
+  
 lemma (in rga) insert_msg_id:
   assumes "Broadcast (i, Insert e n) \<in> set (history j)"
   shows "fst e = i"
-  apply(subgoal_tac "\<exists>state. (i, Insert e n) \<in> valid_rga_msgs j state")
-  defer
-  using assms broadcast_is_valid apply blast
-  apply(erule exE)
-  apply(unfold valid_rga_msgs_def)
-  apply(clarsimp)
-  apply(case_tac n)
-  apply(simp, simp)
-done
+proof -
+  obtain state where 1: "valid_rga_msg state (i, Insert e n)"
+    using assms broadcast_is_valid by blast
+  thus "fst e = i"
+    by(clarsimp simp add: valid_rga_msg_def split: option.split_asm)
+qed
 
 lemma (in rga) allowed_insert:
   assumes "Broadcast (i, Insert e n) \<in> set (history j)"
   shows "n = None \<or> (\<exists>i' e' n'. n = Some (fst e') \<and> Deliver (i', Insert e' n') \<sqsubset>\<^sup>j Broadcast (i, Insert e n))"
-  apply(subgoal_tac "\<exists>pre. pre @ [Broadcast (i, Insert e n)] prefix of j")
-  defer
-  apply(simp add: assms events_before_exist)
-  apply(erule exE)
-  apply(subgoal_tac "\<exists>state. apply_operations pre = Some state \<and> (i, Insert e n) \<in> valid_rga_msgs j state")
-  defer
-  apply(simp add: broadcast_only_valid_msgs)
-  apply(erule exE, erule conjE)
-  apply(unfold valid_rga_msgs_def)
-  apply(case_tac n)
-  apply simp+
-  apply(subgoal_tac "a \<in> element_ids state")
-  defer
-  using apply_opers_idx_elems apply blast
-  apply(subgoal_tac "\<exists>i' v' f' n'. Deliver (i', Insert (a, v', f') n') \<in> set pre")
-  defer
-  using deliver_insert_exists apply blast
-  using events_in_local_order apply blast
-done
-
+proof -
+  obtain pre where 1: "pre @ [Broadcast (i, Insert e n)] prefix of j"
+    using assms events_before_exist by blast
+  from this obtain state where 2: "apply_operations pre = Some state" and 3: "valid_rga_msg state (i, Insert e n)"
+    using broadcast_only_valid_msgs by blast
+  show "n = None \<or> (\<exists>i' e' n'. n = Some (fst e') \<and> Deliver (i', Insert e' n') \<sqsubset>\<^sup>j Broadcast (i, Insert e n))"
+  proof(cases n)
+    fix a
+    assume 4: "n = Some a"
+    hence "a \<in> element_ids state" and 5: "fst e = i"
+      using 3 by(clarsimp simp add: valid_rga_msg_def)+
+    from this have "\<exists>i' v' f' n'. Deliver (i', Insert (a, v', f') n') \<in> set pre"
+      using deliver_insert_exists 2 1 by blast
+    thus "n = None \<or> (\<exists>i' e' n'. n = Some (fst e') \<and> Deliver (i', Insert e' n') \<sqsubset>\<^sup>j Broadcast (i, Insert e n))"
+      using events_in_local_order 1 4 5 by(metis fst_conv)
+  qed simp
+qed
+    
 lemma (in rga) allowed_delete:
   assumes "Broadcast (i, Delete x) \<in> set (history j)"
   shows "\<exists>i' n' v b. Deliver (i', Insert (x, v, b) n') \<sqsubset>\<^sup>j Broadcast (i, Delete x)"
-  apply(subgoal_tac "\<exists>pre. pre @ [Broadcast (i, Delete x)] prefix of j")
-  defer
-  apply(simp add: assms events_before_exist)
-  apply(erule exE)
-  apply(subgoal_tac "\<exists>state. apply_operations pre = Some state \<and> (i, Delete x) \<in> valid_rga_msgs j state")
-  defer
-  apply(simp add: broadcast_only_valid_msgs)
-  apply(erule exE, erule conjE)
-  apply(unfold valid_rga_msgs_def)
-  apply(subgoal_tac "x \<in> element_ids state")
-  defer
-  using apply_opers_idx_elems apply simp
-  apply(subgoal_tac "\<exists>i' v' f' n'. Deliver (i', Insert (x, v', f') n') \<in> set pre")
-  defer
-  using deliver_insert_exists apply blast
-  using events_in_local_order apply blast
-done
+proof -
+  obtain pre where 1: "pre @ [Broadcast (i, Delete x)] prefix of j"
+    using assms events_before_exist by blast
+  from this obtain state where 2: "apply_operations pre = Some state"
+      and "valid_rga_msg state (i, Delete x)"
+    using broadcast_only_valid_msgs by blast
+  hence "x \<in> element_ids state"
+    using apply_opers_idx_elems by(simp add: valid_rga_msg_def)
+  hence "\<exists>i' v' f' n'. Deliver (i', Insert (x, v', f') n') \<in> set pre"
+    using deliver_insert_exists 1 2 by blast
+  thus "\<exists>i' n' v b. Deliver (i', Insert (x, v, b) n') \<sqsubset>\<^sup>j Broadcast (i, Delete x)"
+    using events_in_local_order 1 by blast
+qed
 
 lemma (in rga) insert_id_unique:
   assumes "fst e1 = fst e2"
@@ -209,18 +211,26 @@ by(metis (no_types, lifting) Un_insert_right insert_iff list.simps(15) assms
 lemma (in rga) allowed_insert_deliver:
   assumes "Deliver (i, Insert e n) \<in> set (history j)"
   shows   "n = None \<or> (\<exists>i' n' n'' v b. n = Some n' \<and> Deliver (i', Insert (n', v, b) n'') \<sqsubset>\<^sup>j Deliver (i, Insert e n))"
-using assms
-  apply -
-  apply(frule delivery_has_a_cause)
-  apply(erule exE)
-  apply(cases n; clarsimp)
-  apply(frule allowed_insert)
-  apply clarsimp
-  apply(frule local_order_carrier_closed)
-  apply clarsimp
-  apply(frule delivery_has_a_cause, clarsimp, drule causal_broadcast[rotated, where j=j])
-  apply auto
-done
+proof -
+  obtain ja where 1: "Broadcast (i, Insert e n) \<in> set (history ja)"
+    using assms delivery_has_a_cause by blast
+  show "n = None \<or> (\<exists>i' n' n'' v b. n = Some n' \<and> Deliver (i', Insert (n', v, b) n'') \<sqsubset>\<^sup>j Deliver (i, Insert e n))"
+  proof(cases n)
+    fix a
+    assume 3: "n = Some a"
+    from this obtain i' e' n' where 4: "Some a = Some (fst e')" and
+        2: "Deliver (i', Insert e' n') \<sqsubset>\<^sup>ja Broadcast (i, Insert e (Some a))"
+      using allowed_insert 1 by blast
+    hence "Deliver (i', Insert e' n') \<in> set (history ja)" and "Broadcast (i, Insert e (Some a)) \<in> set (history ja)"
+      using local_order_carrier_closed by simp+
+    from this obtain jaa where "Broadcast (i, Insert e (Some a)) \<in> set (history jaa)"
+      using delivery_has_a_cause by simp
+    have "\<exists>i' n' n'' v b. n = Some n' \<and> Deliver (i', Insert (n', v, b) n'') \<sqsubset>\<^sup>j Deliver (i, Insert e n)"
+      using 2 3 4 by(metis assms causal_broadcast prod.collapse)
+    thus "n = None \<or> (\<exists>i' n' n'' v b. n = Some n' \<and> Deliver (i', Insert (n', v, b) n'') \<sqsubset>\<^sup>j Deliver (i, Insert e n))"
+      by auto
+  qed simp
+qed
 
 lemma (in rga) allowed_insert_deliver_in_set:
   assumes "(es@[Deliver (i, Insert e m)]) prefix of j"
@@ -239,25 +249,24 @@ lemma (in rga) delete_no_failure:
   assumes "es @ [Deliver (i, Delete n)] prefix of j"
       and "apply_operations es = Some s"
     shows "\<exists>ys. delete s n = Some ys"
-using assms 
-  apply -
-  apply(frule allowed_delete_deliver_in_set)
-  apply clarsimp
-  apply(rule delete_no_failure)
-  apply(drule idx_in_elem_inserted)
-  apply(metis apply_opers_idx_elems element_ids_def prefix_of_appendD prod.sel(1) set_map)
-done
+proof -
+  obtain i' na v b where 1: "Deliver (i', Insert (n, v, b) na) \<in> set es"
+    using assms allowed_delete_deliver_in_set by blast
+  also have "fst (n, v, b) \<in> set (indices es)"
+    using assms idx_in_elem_inserted calculation by blast
+  from this assms and 1 show "\<exists>ys. delete s n = Some ys"
+    apply -
+    apply(rule delete_no_failure)
+    apply(metis apply_opers_idx_elems element_ids_def prefix_of_appendD prod.sel(1) set_map)
+    done
+qed
 
 lemma (in rga) Insert_equal:
   assumes "fst e1 = fst e2"
       and "Broadcast (i1, Insert e1 n1) \<in> set (history i)"
       and "Broadcast (i2, Insert e2 n2) \<in> set (history j)"
     shows "Insert e1 n1 = Insert e2 n2"
-using assms
-  apply(subgoal_tac "e1 = e2")
-  apply(metis insert_id_unique)
-  apply(cases e1, cases e2; clarsimp)
-  using insert_id_unique by force
+using insert_id_unique assms by simp
 
 lemma (in rga) same_insert:
   assumes "fst e1 = fst e2"
@@ -265,29 +274,30 @@ lemma (in rga) same_insert:
       and "(i1, Insert e1 n1) \<in> set (node_deliver_messages xs)"
       and "(i2, Insert e2 n2) \<in> set (node_deliver_messages xs)"
     shows "Insert e1 n1 = Insert e2 n2"
-using assms
-  apply -
-  apply(subgoal_tac "Deliver (i1, Insert e1 n1) \<in> set (history i)")
-  apply(subgoal_tac "Deliver (i2, Insert e2 n2) \<in> set (history i)")
-  apply(subgoal_tac "\<exists>j. Broadcast (i1, Insert e1 n1) \<in> set (history j)")
-  apply(subgoal_tac "\<exists>j. Broadcast (i2, Insert e2 n2) \<in> set (history j)")
-  apply(erule exE)+
-  apply(rule Insert_equal, force, force, force) 
-  apply(simp add: delivery_has_a_cause)
-  apply(simp add: delivery_has_a_cause)
-  apply(auto simp add: node_deliver_messages_def prefix_msg_in_history)
-done
-
+proof -
+  have "Deliver (i1, Insert e1 n1) \<in> set (history i)"
+    using assms by(auto simp add: node_deliver_messages_def prefix_msg_in_history)
+  from this obtain j where 1: "Broadcast (i1, Insert e1 n1) \<in> set (history j)"
+    using delivery_has_a_cause by blast
+  have "Deliver (i2, Insert e2 n2) \<in> set (history i)"
+    using assms by(auto simp add: node_deliver_messages_def prefix_msg_in_history)
+  from this obtain k where 2: "Broadcast (i2, Insert e2 n2) \<in> set (history k)"
+    using delivery_has_a_cause by blast
+  show "Insert e1 n1 = Insert e2 n2"
+    by(rule Insert_equal; force simp add: assms intro: 1 2)
+qed
+  
 lemma (in rga) insert_commute_assms:
   assumes "{Deliver (i, Insert e n), Deliver (i', Insert e' n')} \<subseteq> set (history j)"
       and "hb.concurrent (i, Insert e n) (i', Insert e' n')"
     shows "n = None \<or> n \<noteq> Some (fst e')"
 using assms
   apply(clarsimp simp: hb.concurrent_def)
-  apply(case_tac e')
+  apply(cases e')
   apply clarsimp
   apply(frule delivery_has_a_cause)
-  apply(frule delivery_has_a_cause, clarsimp, frule allowed_insert)
+  apply(frule delivery_has_a_cause, clarsimp)
+  apply(frule allowed_insert)
   apply clarsimp
   apply(metis Insert_equal delivery_has_a_cause fst_conv hb.intros(2) insert_subset
     local_order_carrier_closed insert_msg_id)
@@ -302,12 +312,13 @@ lemma (in rga) Insert_Insert_concurrent:
   assumes "{Deliver (i, Insert e k), Deliver (i', Insert e' (Some m))} \<subseteq> set (history j)"
       and "hb.concurrent (i, Insert e k) (i', Insert e' (Some m))"
     shows "fst e \<noteq> m"
-by(metis assms subset_reorder hb.concurrent_comm insert_commute_assms option.simps(3))
+  by(metis assms subset_reorder hb.concurrent_comm insert_commute_assms option.simps(3))
 
 lemma (in rga) insert_valid_assms:
  assumes "Deliver (i, Insert e n) \<in> set (history j)"
    shows "n = None \<or> n \<noteq> Some (fst e)"
-using assms by(meson allowed_insert_deliver hb.concurrent_def hb.less_asym insert_subset local_order_carrier_closed rga.insert_commute_assms rga_axioms)
+  using assms by(meson allowed_insert_deliver hb.concurrent_def hb.less_asym insert_subset
+      local_order_carrier_closed rga.insert_commute_assms rga_axioms)
 
 lemma (in rga) Insert_Delete_concurrent:
   assumes "{Deliver (i, Insert e n), Deliver (i', Delete n')} \<subseteq> set (history j)"
@@ -316,67 +327,97 @@ lemma (in rga) Insert_Delete_concurrent:
 by (metis assms Insert_equal allowed_delete delivery_has_a_cause fst_conv hb.concurrent_def
   hb.intros(2) insert_subset local_order_carrier_closed rga.insert_msg_id rga_axioms)
 
-lemma (in rga) apply_operations_distinct:
-  assumes "xs prefix of i"
-      and "apply_operations xs = Some ys"
-    shows "distinct (map fst ys)"
-oops
-
 lemma (in rga) concurrent_operations_commute:
   assumes "xs prefix of i"
   shows "hb.concurrent_ops_commute (node_deliver_messages xs)"
-using assms
-  apply(clarsimp simp: hb.concurrent_ops_commute_def)
-  apply(rule ext)
-  apply(simp add: kleisli_def interp_msg_def)
-  apply(case_tac b; case_tac ba)
-  apply clarsimp
-  apply(case_tac "ab = ad")
-  apply(subgoal_tac "(ab, ac, bb) = (ad, ae, bc) \<and> x12a = x12")
-  apply force
-  defer
-  apply(subgoal_tac "Ordered_List.insert x (ab, ac, bb) x12 \<bind> (\<lambda>x. Ordered_List.insert x (ad, ae, bc) x12a) = Ordered_List.insert x (ad, ae, bc) x12a \<bind> (\<lambda>x. Ordered_List.insert x (ab, ac, bb) x12)")
-  apply(metis (no_types, lifting) Option.bind_cong interpret_opers.simps(1))
-  apply(rule insert_commutes)
-  apply simp
-  prefer 2
-  apply(subst (asm) hb.concurrent_comm)
-  apply(rule insert_commute_assms)
-  prefer 2
-  apply assumption
-  apply clarsimp
-  apply(rule conjI)
-  apply(rule prefix_msg_in_history, assumption, force)
-  apply(rule prefix_msg_in_history, assumption, force)
-  apply(rule insert_commute_assms)
-  prefer 2
-  apply assumption
-  apply clarsimp
-  apply(rule conjI)
-  apply(rule prefix_msg_in_history, assumption, force)
-  apply(rule prefix_msg_in_history, assumption, force)
-  apply(clarsimp simp del: delete.simps)
-  apply(subgoal_tac "Ordered_List.insert x (ab, ac, bb) x12 \<bind> (\<lambda>x. Ordered_List.delete x x2) = delete x x2 \<bind> (\<lambda>x. Ordered_List.insert x (ab, ac, bb) x12)")
-  apply(metis (no_types, lifting) Option.bind_cong interpret_opers.simps)
-  apply(rule insert_delete_commute)
-  apply(rule Insert_Delete_concurrent)
-  apply clarsimp
-  using prefix_msg_in_history apply blast
-  apply(clarsimp)
-  apply(clarsimp simp del: delete.simps)
-  apply(subgoal_tac "delete x x2 \<bind> (\<lambda>x. insert x (ab, ac, bb) x12) = Ordered_List.insert x (ab, ac, bb) x12 \<bind> (\<lambda>x. delete x x2)")
-  apply(metis (no_types, lifting) Option.bind_cong interpret_opers.simps)
-  apply(rule insert_delete_commute[symmetric])
-  apply(rule Insert_Delete_concurrent)
-  using prefix_msg_in_history apply blast
-  apply(subst (asm) hb.concurrent_comm)
-  apply assumption
-  apply(clarsimp simp del: delete.simps)
-  apply(subgoal_tac "delete x x2 \<bind> (\<lambda>x. delete x x2a) = delete x x2a \<bind> (\<lambda>x. delete x x2)")
-  apply(metis (mono_tags, lifting) Option.bind_cong interpret_opers.simps(2))
-  apply(rule delete_commutes)
-  using same_insert apply force
-done
+proof -
+  have "\<And>x y. {x, y} \<subseteq> set (node_deliver_messages xs) \<Longrightarrow> hb.concurrent x y \<Longrightarrow> interp_msg x \<rhd> interp_msg y = interp_msg y \<rhd> interp_msg x"
+  proof
+    fix x y ii
+    assume "{x, y} \<subseteq> set (node_deliver_messages xs)"
+      and C: "hb.concurrent x y"
+    hence X: "x \<in> set (node_deliver_messages xs)" and Y: "y \<in> set (node_deliver_messages xs)"
+      by auto
+    obtain x1 x2 y1 y2 where 1: "x = (x1, x2)" and 2: "y = (y1, y2)"
+      by fastforce
+    have "(interp_msg (x1, x2) \<rhd> interp_msg (y1, y2)) ii = (interp_msg (y1, y2) \<rhd> interp_msg (x1, x2)) ii"
+    proof(cases x2; cases y2)
+      fix ix1 ix2 iy1 iy2
+      assume X2: "x2 = Insert ix1 ix2" and Y2: "y2 = Insert iy1 iy2"
+      show "(interp_msg (x1, x2) \<rhd> interp_msg (y1, y2)) ii = (interp_msg (y1, y2) \<rhd> interp_msg (x1, x2)) ii"
+      proof(cases "fst ix1 = fst iy1")
+        assume "fst ix1 = fst iy1"
+        hence "Insert ix1 ix2 = Insert iy1 iy2"
+          apply(rule same_insert)
+          using 1 2 X Y X2 Y2 assms apply auto
+          done
+        hence "ix1 = iy1" and "ix2 = iy2"
+          by auto
+        from this and X2 Y2 show "(interp_msg (x1, x2) \<rhd> interp_msg (y1, y2)) ii = (interp_msg (y1, y2) \<rhd> interp_msg (x1, x2)) ii"
+          by(clarsimp simp add: kleisli_def interp_msg_def)
+      next
+        assume NEQ: "fst ix1 \<noteq> fst iy1"
+        have "ix2 = None \<or> ix2 \<noteq> Some (fst iy1)"
+          apply(rule insert_commute_assms)
+          using prefix_msg_in_history[OF assms] X Y X2 Y2 1 2
+           apply(clarsimp, blast)
+          using C 1 2 X2 Y2 apply blast
+          done
+        also have "iy2 = None \<or> iy2 \<noteq> Some (fst ix1)"
+          apply(rule insert_commute_assms)
+          using prefix_msg_in_history[OF assms] X Y X2 Y2 1 2
+           apply(clarsimp, blast)
+          using "1" "2" C X2 Y2 apply blast
+          done
+        ultimately have "insert ii ix1 ix2 \<bind> (\<lambda>x. insert x iy1 iy2) = insert ii iy1 iy2 \<bind> (\<lambda>x. insert x ix1 ix2)"
+          using NEQ insert_commutes by blast
+        thus "(interp_msg (x1, x2) \<rhd> interp_msg (y1, y2)) ii = (interp_msg (y1, y2) \<rhd> interp_msg (x1, x2)) ii"
+          by(clarsimp simp add: interp_msg_def X2 Y2 kleisli_def)
+      qed
+    next
+      fix ix1 ix2 yd
+      assume X2: "x2 = Insert ix1 ix2" and Y2: "y2 = Delete yd"
+      have "hb.concurrent (x1, Insert ix1 ix2) (y1, Delete yd)"
+        using C X2 Y2 1 2 by simp
+      also have "{Deliver (x1, Insert ix1 ix2), Deliver (y1, Delete yd)} \<subseteq> set (history i)"
+        using prefix_msg_in_history assms X2 Y2 X Y 1 2 by blast
+      ultimately have "yd \<noteq> fst ix1"
+        apply -
+        apply(rule Insert_Delete_concurrent; force)
+        done
+      hence "insert ii ix1 ix2 \<bind> (\<lambda>x. delete x yd) = delete ii yd \<bind> (\<lambda>x. insert x ix1 ix2)"
+        by(rule insert_delete_commute)
+      thus "(interp_msg (x1, x2) \<rhd> interp_msg (y1, y2)) ii = (interp_msg (y1, y2) \<rhd> interp_msg (x1, x2)) ii"
+        by(clarsimp simp add: interp_msg_def kleisli_def X2 Y2)
+    next
+      fix xd iy1 iy2
+      assume X2: "x2 = Delete xd" and Y2: "y2 = Insert iy1 iy2"
+      have "hb.concurrent (x1, Delete xd) (y1, Insert iy1 iy2)"
+        using C X2 Y2 1 2 by simp
+      also have "{Deliver (x1, Delete xd), Deliver (y1, Insert iy1 iy2)} \<subseteq> set (history i)"
+        using prefix_msg_in_history assms X2 Y2 X Y 1 2 by blast
+      ultimately have "xd \<noteq> fst iy1"
+        apply -
+        apply(rule Insert_Delete_concurrent; force)
+        done
+      hence "delete ii xd \<bind> (\<lambda>x. insert x iy1 iy2) = insert ii iy1 iy2 \<bind> (\<lambda>x. delete x xd)"
+        by(rule insert_delete_commute[symmetric])
+      thus "(interp_msg (x1, x2) \<rhd> interp_msg (y1, y2)) ii = (interp_msg (y1, y2) \<rhd> interp_msg (x1, x2)) ii"
+        by(clarsimp simp add: interp_msg_def kleisli_def X2 Y2)
+    next
+      fix xd yd
+      assume X2: "x2 = Delete xd" and Y2: "y2 = Delete yd"
+      have "delete ii xd \<bind> (\<lambda>x. delete x yd) = delete ii yd \<bind> (\<lambda>x. delete x xd)"
+        by(rule delete_commutes)
+      thus "(interp_msg (x1, x2) \<rhd> interp_msg (y1, y2)) ii = (interp_msg (y1, y2) \<rhd> interp_msg (x1, x2)) ii"
+        by(clarsimp simp add: interp_msg_def kleisli_def X2 Y2)
+    qed   
+    thus "(interp_msg x \<rhd> interp_msg y) ii = (interp_msg y \<rhd> interp_msg x) ii"
+      using 1 2 by auto
+  qed
+  thus "hb.concurrent_ops_commute (node_deliver_messages xs)"
+    by(auto simp add: hb.concurrent_ops_commute_def)
+qed
 
 corollary (in rga) concurrent_operations_commute':
   shows "hb.concurrent_ops_commute (node_deliver_messages (history i))"
@@ -385,29 +426,63 @@ by (meson concurrent_operations_commute append.right_neutral prefix_of_node_hist
 lemma (in rga) apply_operations_never_fails:
   assumes "xs prefix of i"
   shows "apply_operations xs \<noteq> None"
-  using assms
-  apply(induction xs rule: rev_induct)
-   apply clarsimp
-  apply(case_tac "x"; clarsimp)
-   apply force
-  apply(case_tac "b"; clarsimp)
-  apply(metis bind.bind_lunit interpret_opers.simps(1) prefix_of_appendD rga.Insert_no_failure
-    rga_axioms interp_msg_def prod.sel(2))
-  apply(metis bind.bind_lunit interpret_opers.simps(2) local.delete_no_failure prefix_of_appendD
-    interp_msg_def prod.sel(2))
-done
+using assms proof(induction xs rule: rev_induct)
+  show "apply_operations [] \<noteq> None"
+    by clarsimp
+next
+  fix x xs
+  assume 1: "xs prefix of i \<Longrightarrow> apply_operations xs \<noteq> None"
+    and 2: "xs @ [x] prefix of i"
+  hence 3: "xs prefix of i"
+    by auto
+  show "apply_operations (xs @ [x]) \<noteq> None"
+  proof(cases x)
+    fix b
+    assume "x = Broadcast b"
+    thus "apply_operations (xs @ [x]) \<noteq> None"
+      using 1 3 by clarsimp
+  next
+    fix d
+    assume 4: "x = Deliver d"
+    thus "apply_operations (xs @ [x]) \<noteq> None"
+    proof(cases d; clarify)
+      fix a b
+      assume 5: "x = Deliver (a, b)"
+      show "\<exists>y. apply_operations (xs @ [Deliver (a, b)]) = Some y"
+      proof(cases b; clarify)
+        fix aa aaa ba x12
+        assume 6: "b = Insert (aa, aaa, ba) x12"
+        show "\<exists>y. apply_operations (xs @ [Deliver (a, Insert (aa, aaa, ba) x12)]) = Some y"
+          apply(clarsimp simp add: 1 interp_msg_def split!: bind_splits)
+           apply(simp add: "1" "3")
+          apply(rule rga.Insert_no_failure, rule rga_axioms)
+          using 4 5 6 2 apply force+
+          done
+      next
+        fix x2
+        assume 6: "b = Delete x2"
+        show "\<exists>y. apply_operations (xs @ [Deliver (a, Delete x2)]) = Some y"
+          apply(clarsimp simp add: interp_msg_def split!: bind_splits)
+           apply(simp add: 1 3)
+          apply(rule delete_no_failure)
+          using 4 5 6 2 apply force+
+          done
+      qed
+    qed
+  qed
+qed
 
 lemma (in rga) apply_operations_never_fails':
   shows "apply_operations (history i) \<noteq> None"
-by (meson apply_operations_never_fails append.right_neutral prefix_of_node_history_def)
+by(meson apply_operations_never_fails append.right_neutral prefix_of_node_history_def)
 
 corollary (in rga) rga_convergence:
   assumes "set (node_deliver_messages xs) = set (node_deliver_messages ys)"
       and "xs prefix of i"
       and "ys prefix of j"
     shows "apply_operations xs = apply_operations ys"
-using assms by(auto simp add: apply_operations_def intro: hb.convergence_ext concurrent_operations_commute
-                node_deliver_messages_distinct hb_consistent_prefix)
+  using assms by(auto simp add: apply_operations_def intro: hb.convergence_ext
+      concurrent_operations_commute node_deliver_messages_distinct hb_consistent_prefix)
 
 subsection\<open>Strong eventual consistency\<close>
               
@@ -415,17 +490,41 @@ context rga begin
 
 sublocale sec: strong_eventual_consistency weak_hb hb interp_msg
   "\<lambda>ops.\<exists>xs i. xs prefix of i \<and> node_deliver_messages xs = ops" "[]"
-  apply(standard; clarsimp)
-      apply(auto simp add: hb_consistent_prefix node_deliver_messages_distinct
-        concurrent_operations_commute apply_operations_def)
-   apply(metis (no_types, lifting) apply_operations_def bind.bind_lunit not_None_eq
-     hb.apply_operations_Snoc kleisli_def apply_operations_never_fails interp_msg_def)
-  using drop_last_message apply blast
-  done
+proof(standard; clarsimp)
+  fix xsa i
+  assume "xsa prefix of i"
+  thus "hb.hb_consistent (node_deliver_messages xsa)"
+    by(auto simp add: hb_consistent_prefix)
+next
+  fix xsa i
+  assume "xsa prefix of i"
+  thus "distinct (node_deliver_messages xsa)"
+    by(auto simp add: node_deliver_messages_distinct)
+next
+  fix xsa i
+  assume "xsa prefix of i"
+  thus "hb.concurrent_ops_commute (node_deliver_messages xsa)"
+    by(auto simp add: concurrent_operations_commute)
+next
+  fix xs a b state xsa x
+  assume "hb.apply_operations xs [] = Some state"
+    and "node_deliver_messages xsa = xs @ [(a, b)]"
+    and "xsa prefix of x"
+  thus "\<exists>y. interp_msg (a, b) state = Some y"
+   by(metis (no_types, lifting) apply_operations_def bind.bind_lunit not_None_eq
+       hb.apply_operations_Snoc kleisli_def apply_operations_never_fails interp_msg_def)
+next
+  fix xs a b xsa x
+  assume "node_deliver_messages xsa = xs @ [(a, b)]"
+    and "xsa prefix of x"
+  thus "\<exists>xsa. (\<exists>x. xsa prefix of x) \<and> node_deliver_messages xsa = xs"
+    using drop_last_message by blast
+qed
 
 end
   
 interpretation trivial_rga_implementation: rga "\<lambda>x. []"
-  by (standard, auto simp add: trivial_node_histories.history_order_def trivial_node_histories.prefix_of_node_history_def)
+  by(standard, auto simp add: trivial_node_histories.history_order_def
+      trivial_node_histories.prefix_of_node_history_def)
 
 end
