src/Counter.thy
@@ -1,6 +1,7 @@
 (* Victor B. F. Gomes, University of Cambridge
    Martin Kleppmann, University of Cambridge
    Dominic P. Mulligan, University of Cambridge
+   Alastair R. Beresford, University of Cambridge
 *)
 
 section\<open>Increment-Decrement Counter\<close>
@@ -19,8 +20,6 @@ datatype operation = Increment | Decrement
 fun counter_op :: "operation \<Rightarrow> int \<rightharpoonup> int" where
   "counter_op Increment x = Some (x + 1)" |
   "counter_op Decrement x = Some (x - 1)"
-  
-export_code Increment counter_op in OCaml file "ocaml/counter.ml"
 
 locale counter = network_with_ops _ counter_op 0
 
@@ -32,28 +31,27 @@ lemma (in counter) concurrent_operations_commute:
   shows "hb.concurrent_ops_commute (node_deliver_messages xs)"
   using assms
   apply(clarsimp simp: hb.concurrent_ops_commute_def)
-  apply(unfold interp_msg_def, simp)
-  apply(case_tac "b"; case_tac "ba")
-   apply(auto simp add: kleisli_def)
-done
+  apply(rename_tac a b x y)
+  apply(case_tac b; case_tac y; force simp add: interp_msg_def kleisli_def)
+  done
   
 corollary (in counter) counter_convergence:
   assumes "set (node_deliver_messages xs) = set (node_deliver_messages ys)"
       and "xs prefix of i"
       and "ys prefix of j"
     shows "apply_operations xs = apply_operations ys"
-using assms by(auto simp add: apply_operations_def intro: hb.convergence_ext concurrent_operations_commute
-                node_deliver_messages_distinct hb_consistent_prefix)
+  using assms by(auto simp add: apply_operations_def intro: hb.convergence_ext
+      concurrent_operations_commute node_deliver_messages_distinct hb_consistent_prefix)
 
 context counter begin
 
 sublocale sec: strong_eventual_consistency weak_hb hb interp_msg
   "\<lambda>ops. \<exists>xs i. xs prefix of i \<and> node_deliver_messages xs = ops" 0
-  apply(standard; clarsimp)
-      apply(auto simp add: hb_consistent_prefix drop_last_message node_deliver_messages_distinct concurrent_operations_commute)
+  apply(standard; clarsimp simp add: hb_consistent_prefix drop_last_message
+      node_deliver_messages_distinct concurrent_operations_commute)
    apply(metis (full_types) interp_msg_def counter_op.elims)
   using drop_last_message apply blast
-done
+  done
 
 end
 end
