src/Util.thy
@@ -1,6 +1,7 @@
 (* Victor B. F. Gomes, University of Cambridge
    Martin Kleppmann, University of Cambridge
    Dominic P. Mulligan, University of Cambridge
+   Alastair R. Beresford, University of Cambridge
 *)
 
 section\<open>Technical Lemmas\<close>
@@ -12,7 +13,7 @@ theory
   Util
 imports
   Main
-  "~~/src/HOL/Library/Monad_Syntax"
+  "HOL-Library.Monad_Syntax"
 begin
 
 subsection\<open>Kleisli arrow composition\<close>
@@ -23,81 +24,49 @@ definition kleisli :: "('b \<Rightarrow> 'b option) \<Rightarrow> ('b \<Rightarr
 lemma kleisli_comm_cong:
   assumes "x \<rhd> y = y \<rhd> x"
   shows   "z \<rhd> x \<rhd> y = z \<rhd> y \<rhd> x"
-using assms by(clarsimp simp add: kleisli_def)
+  using assms by(clarsimp simp add: kleisli_def)
 
 lemma kleisli_assoc:
   shows "(z \<rhd> x) \<rhd> y = z \<rhd> (x \<rhd> y)"
-by(auto simp add: kleisli_def)
+  by(auto simp add: kleisli_def)
 
 subsection\<open>Lemmas about sets\<close>
 
 lemma distinct_set_notin [dest]:
   assumes "distinct (x#xs)"
   shows   "x \<notin> set xs"
-using assms by(induction xs, auto)
+  using assms by(induction xs, auto)
 
 lemma set_membership_equality_technicalD [dest]:
   assumes "{x} \<union> (set xs) = {y} \<union> (set ys)"
-    shows "x = y \<or> y \<in> set xs"
-using assms by(induction xs, auto)
+  shows "x = y \<or> y \<in> set xs"
+  using assms by(induction xs, auto)
 
 lemma set_equality_technical:
   assumes "{x} \<union> (set xs) = {y} \<union> (set ys)"
       and "x \<notin> set xs"
       and "y \<notin> set ys"
       and "y \<in> set xs"
-  shows "{x} \<union> (set xs - {y}) = set ys"
-using assms by (induction xs) auto
+    shows "{x} \<union> (set xs - {y}) = set ys"
+  using assms by (induction xs) auto
     
 lemma set_elem_nth:
   assumes "x \<in> set xs"
   shows   "\<exists>m. m < length xs \<and> xs ! m = x"
   using assms by(induction xs, simp) (meson in_set_conv_nth)
-
-subsection\<open>Lemmas about nondeterministic choice and let\<close>
-
-lemma unpack_let:
-  assumes "(let x = y in f x) = z"
-  and "\<And>x. x = y \<Longrightarrow> f x = z \<Longrightarrow> R"
-  shows R
-using assms by auto
-
-lemma some_set_memb:
-  assumes "y \<noteq> {}"
-  shows "(SOME x. x \<in> y) \<in> y"
-by (rule someI_ex, simp add: assms ex_in_conv)
-
-lemma choose_set_memb:
-  assumes "y \<noteq> {}"
-  and "x = (SOME x. x \<in> y)"
-  shows "x \<in> y"
-using assms by (simp add: some_set_memb)
-
-lemma let_some_elim:
-  assumes "(let x = (SOME x. P x) in f x) = z"
-    and "\<exists>x. P x"
-    and "\<And>x. P x \<Longrightarrow> f x = z \<Longrightarrow> R"
-  shows R
-  using assms by (metis someI)
-
-lemma let_some_set_elim:
-  assumes "(let x = (SOME x'. x' \<in> y) in f x) = z"
-  and "y \<noteq> {}"
-  and "\<And>x. (x \<in> y \<and> f x = z) \<Longrightarrow> R"
-  shows R
-by (metis assms some_set_memb)
-
+    
 subsection\<open>Lemmas about list\<close>
 
 lemma list_nil_or_snoc:
   shows "xs = [] \<or> (\<exists>y ys. xs = ys@[y])"
-by (induction xs, auto)
+  by (induction xs, auto)
 
 lemma suffix_eq_distinct_list:
-  assumes "ys@suf1 = xs"
+  assumes "distinct xs"
+      and "ys@suf1 = xs"
       and "ys@suf2 = xs"
     shows "suf1 = suf2"
-using assms by(induction xs arbitrary: suf1 suf2 rule: rev_induct, simp) (metis append_eq_append_conv)
+  using assms by(induction xs arbitrary: suf1 suf2 rule: rev_induct, simp) (metis append_eq_append_conv)
 
 lemma pre_suf_eq_distinct_list:
   assumes "distinct xs"
@@ -108,11 +77,11 @@ lemma pre_suf_eq_distinct_list:
 using assms
   apply(induction xs arbitrary: pre1 pre2 ys, simp)
   apply(case_tac "pre1"; case_tac "pre2"; clarify)
-  apply(metis suffix_eq_distinct_list append_Nil)
+   apply(metis suffix_eq_distinct_list append_Nil)
   apply(metis Un_iff append_eq_Cons_conv distinct.simps(2) list.set_intros(1) set_append suffix_eq_distinct_list)
   apply(metis Un_iff append_eq_Cons_conv distinct.simps(2) list.set_intros(1) set_append suffix_eq_distinct_list)
   apply(metis distinct.simps(2) hd_append2 list.sel(1) list.sel(3) list.simps(3) tl_append2)
-done
+  done
 
 lemma list_head_unaffected:
   assumes "hd (x @ [y, z]) = v"
@@ -129,114 +98,58 @@ lemma list_head_length_one:
   assumes "hd xs = x"
     and "length xs = 1"
   shows "xs = [x]"
-using assms by(metis One_nat_def Suc_length_conv hd_Cons_tl length_0_conv list.sel(3))
+  using assms by(metis One_nat_def Suc_length_conv hd_Cons_tl length_0_conv list.sel(3))
 
 lemma list_two_at_end:
   assumes "length xs > 1"
   shows "\<exists>xs' x y. xs = xs' @ [x, y]"
-  using assms apply(induction xs rule: rev_induct, simp)
+  using assms
+  apply(induction xs rule: rev_induct, simp)
   apply(case_tac "length xs = 1", simp)
-  apply(rule_tac x="[]" in exI, rule_tac x="hd xs" in exI)
-  apply(simp_all add: list_head_length_one)
+   apply(metis append_self_conv2 length_0_conv length_Suc_conv)
   apply(rule_tac x="butlast xs" in exI, rule_tac x="last xs" in exI, simp)
-done
-
-lemma nth_list_item:
-  assumes "xs = ys @ x # zs"
-  shows "xs ! length ys = x"
-  using assms by simp
+  done
 
 lemma list_nth_split_technical:
   assumes "m < length cs"
       and "cs \<noteq> []"
     shows "\<exists>xs ys. cs = xs@(cs!m)#ys"
-using assms
+  using assms
   apply(induction m arbitrary: cs)
-  apply(meson in_set_conv_decomp nth_mem)
+   apply(meson in_set_conv_decomp nth_mem)
   apply(metis in_set_conv_decomp length_list_update set_swap set_update_memI)
-done
+  done
 
 lemma list_nth_split:
   assumes "m < length cs"
       and "n < m"
       and "1 < length cs"
     shows "\<exists>xs ys zs. cs = xs@(cs!n)#ys@(cs!m)#zs"
-using assms
-  apply(induction n arbitrary: cs m)
-  apply(rule_tac x="[]" in exI, clarsimp)
-  apply(case_tac cs; clarsimp)
-  apply(rule list_nth_split_technical, simp, force)
-  apply(case_tac cs; clarsimp)
-  apply(rename_tac w ws)
-  apply(erule_tac x="ws" in meta_allE, erule_tac x="m-1" in meta_allE)
-  apply(subgoal_tac "m-1 < length ws", subgoal_tac "n<m-1", clarsimp)
-  apply(rule_tac x="w#xs" in exI, rule_tac x="ys" in exI, rule_tac x="zs" in exI)
-  apply force+
-done
-
-lemma split_first_occurrence:
-  assumes "xs = as @ x # bs"
-      and "xs = cs @ x # ds"
-      and "x \<notin> set as" "x \<notin> set cs"
-    shows "as = cs \<and> bs = ds"
-  using assms
-  apply(induction xs arbitrary: as bs cs ds rule: rev_induct, simp)
-  apply (rename_tac y ys as bs cs ds)
-  apply(case_tac "x \<in> set ys")
-  apply(erule_tac x=as in meta_allE, erule_tac x="butlast bs" in meta_allE)
-  apply(erule_tac x=cs in meta_allE, erule_tac x="butlast ds" in meta_allE)
-  apply(simp, rule conjI)
-  apply(metis append_Nil2 butlast.simps(2) butlast_append list.simps(3))
-  apply(metis (no_types, lifting) append_Nil2 append_butlast_last_id
-    butlast.simps(2) butlast_append last.simps last_appendR list.simps(3))
-  apply(case_tac "x = y")
-  apply(erule_tac x=as in meta_allE, erule_tac x="[]" in meta_allE)
-  apply(erule_tac x=cs in meta_allE, erule_tac x="[]" in meta_allE)
-  apply(metis append_Nil2 butlast.simps(2) butlast_append in_set_conv_decomp)
-  apply(subgoal_tac "x \<notin> set (ys @ [y])")
-  apply(metis in_set_conv_decomp)
-  apply(metis butlast.simps(2) butlast_append butlast_snoc in_set_conv_decomp
-    last_snoc list.simps(3))
-done
-
-lemma list_first_index:
-  assumes "x \<in> set xs"
-  shows "\<exists>pre i suf. i < length xs \<and> xs!i = x \<and> xs = pre @ [xs!i] @ suf \<and>
-           x \<notin> set pre \<and> i = length pre"
-  using assms
-  apply(induction xs rule: rev_induct, simp)
-  apply(rename_tac y ys)
-  apply(case_tac "x \<in> set ys")
-  apply(simp, (erule exE)+, (erule conjE)+, erule exE)
-  apply(rule_tac x=pre in exI)
-  apply(rule conjI)
-  using less_Suc_eq apply blast
-  apply(rule conjI, meson nth_append)
-  apply(rule conjI, rule_tac x="suf @ [y]" in exI)
-  apply(metis append_Cons append_eq_appendI nth_append, simp)
-  apply(subgoal_tac "x=y") prefer 2 apply simp
-  apply(rule_tac x=ys in exI, rule_tac x="length ys" in exI)
-  apply(rule_tac x="[]" in exI, simp)
-done
-
-lemma unique_prefix_length:
-  assumes "xs = pre @ xs!i # suf"
-    and "xs!i \<notin> set pre"
-    and "\<forall>j<i. xs!j \<noteq> xs!i"
-    and "i < length xs"
-  shows "i = length pre"
-  using assms
-  apply(induction xs arbitrary: pre suf rule: rev_induct, simp)
-  apply(case_tac "i < length xs")
-  apply(erule_tac x=pre in meta_allE, erule_tac x="butlast suf" in meta_allE)
-  apply(metis in_set_conv_nth nat_neq_iff nth_append nth_append_length)
-  apply(subgoal_tac "i = length xs") defer apply force
-  apply(subgoal_tac "x = (xs @ [x]) ! i") defer apply(metis nth_append_length)
-  apply(simp)
-  apply(case_tac "suf = []", simp)
-  apply(metis (no_types, lifting) One_nat_def add.assoc add_diff_cancel_right' butlast_snoc
-    length_append length_butlast list.size(4) nat_neq_iff not_add_less1 nth_append_length)
-done
+using assms proof(induction n arbitrary: cs m)
+  case 0 thus ?case
+    apply(case_tac cs; clarsimp)
+    apply(rule_tac x="[]" in exI, clarsimp)
+    apply(rule list_nth_split_technical, simp, force)
+    done
+next
+  case (Suc n)
+  thus ?case
+  proof (cases cs)
+    case Nil
+    then show ?thesis
+      using Suc.prems by auto
+  next
+    case (Cons a as)
+    hence "m-1 < length as" "n < m-1"
+      using Suc by force+
+    then obtain xs ys zs where "as = xs @ as ! n # ys @ as ! (m-1) # zs"
+      using Suc by force
+    thus ?thesis
+      apply(rule_tac x="a#xs" in exI) 
+      using Suc Cons apply force
+      done
+   qed
+qed
 
 lemma list_split_two_elems:
   assumes "distinct cs"
@@ -244,98 +157,35 @@ lemma list_split_two_elems:
       and "y \<in> set cs"
       and "x \<noteq> y"
     shows "\<exists>pre mid suf. cs = pre @ x # mid @ y # suf \<or> cs = pre @ y # mid @ x # suf"
-  using assms
-  apply(subgoal_tac "\<exists>xi. xi < length cs \<and> x = cs ! xi")
-  apply(subgoal_tac "\<exists>yi. yi < length cs \<and> y = cs ! yi")
-  apply clarsimp
-  apply(subgoal_tac "xi \<noteq> yi")
-  apply(case_tac "xi < yi")
-  apply(metis list_nth_split One_nat_def less_Suc_eq linorder_neqE_nat not_less_zero)
-  apply(subgoal_tac "yi < xi")
-  apply(metis list_nth_split One_nat_def less_Suc_eq linorder_neqE_nat not_less_zero)
-  using set_elem_nth linorder_neqE_nat apply fastforce+
-done
+proof -
+  obtain xi yi where *: "xi < length cs \<and> x = cs ! xi" "yi < length cs \<and> y = cs ! yi" "xi \<noteq> yi"
+    using set_elem_nth linorder_neqE_nat assms by metis
+  thus ?thesis
+    by (metis list_nth_split One_nat_def less_Suc_eq linorder_neqE_nat not_less_zero)
+qed
 
 lemma split_list_unique_prefix:
   assumes "x \<in> set xs"
   shows "\<exists>pre suf. xs = pre @ x # suf \<and> (\<forall>y \<in> set pre. x \<noteq> y)"
-using assms
-  apply(induction xs; clarsimp)
-  apply(rename_tac a as)
-  apply(case_tac "a = x")
-  apply(rule_tac x="[]" in exI, force)
-  apply(subgoal_tac "x \<in> set xs", clarsimp)
-  apply(rule_tac x="a # pre" in exI)
-  apply force+
-done
+using assms proof(induction xs)
+  case Nil thus ?case by clarsimp
+next
+  case (Cons y ys)
+  then show ?case
+    proof (cases "y=x")
+      case True
+      then show ?thesis by force
+    next
+      case False
+      then obtain pre suf where "ys = pre @ x # suf \<and> (\<forall>y\<in>set pre. x \<noteq> y)"
+        using assms Cons by auto
+      thus ?thesis
+        using split_list_first by force
+    qed
+qed
 
 lemma map_filter_append:
   shows "List.map_filter P (xs @ ys) = List.map_filter P xs @ List.map_filter P ys"
-by(auto simp add: List.map_filter_def)
-
-lemma unique_first_occurrence:
-  assumes "xs = ys1 @ zs1"
-      and "xs = ys2 @ [hd zs1] @ zs2"
-      and "hd zs1 \<notin> set ys1"
-      and "hd zs1 \<notin> set ys2"
-      and "zs1 \<noteq> []"
-    shows "ys1 = ys2 \<and> zs1 = [hd zs1] @ zs2"
-  using assms apply -
-  apply(subgoal_tac "ys1 = ys2", simp)
-  apply(induction zs1 arbitrary: xs zs2 rule: rev_induct, force)
-  apply(case_tac "zs2 = []", simp)
-  using hd_append2 hd_in_set apply force
-  apply(erule_tac x="butlast xsa" in meta_allE)
-  apply(erule_tac x="butlast zs2" in meta_allE)
-  apply(case_tac "xs = []", simp)
-  apply(metis butlast.simps(2) butlast_append butlast_snoc in_set_conv_decomp)
-  apply(metis append_Cons append_Nil2 butlast_append butlast_snoc hd_append2 in_set_conv_decomp)
-done
-
-lemma first_occurrence_length:
-  assumes "xs = ys1 @ zs1"
-      and "xs = ys2 @ zs2"
-      and "hd zs1 \<notin> set ys1"
-      and "hd zs1 \<notin> set ys2"
-      and "zs1 \<noteq> []"
-    shows "length ys2 \<le> length ys1"
-  using assms
-  apply(induction zs1 arbitrary: xs zs2 rule: rev_induct, force)
-  apply(subgoal_tac "hd (xs @ [x]) \<in> set zs2 \<and> hd (xs @ [x]) \<in> set xsa") defer
-  apply(metis Un_iff hd_in_set set_append, erule conjE)
-  apply(case_tac "zs2 = []", simp)
-  apply(erule_tac x="butlast xsa" in meta_allE)
-  apply(erule_tac x="butlast zs2" in meta_allE)
-  apply(case_tac "xs = []", simp)
-  apply(metis in_set_conv_nth not_le nth_append nth_append_length)
-  apply(metis butlast_append butlast_snoc hd_append2)
-done
-
-lemma drop_final_append:
-  assumes "xs = ys1 @ zs1"
-      and "xs = ys2 @ zs2"
-      and "length ys2 \<le> length ys1"
-    shows "\<exists>es. ys2 @ es = ys1 \<and> es @ zs1 = zs2"
-  using assms
-  apply(induction zs1 arbitrary: xs zs2 rule: rev_induct, force)
-  apply(rename_tac z zs2)
-  apply(erule_tac x="butlast z" in meta_allE)
-  apply(erule_tac x="butlast zs2" in meta_allE)
-  apply(subgoal_tac "butlast z = ys1 @ xs") prefer 2
-  apply(simp add: butlast_append)
-  apply(subgoal_tac "butlast z = ys2 @ butlast zs2") prefer 2
-  apply(simp add: append_eq_append_conv_if butlast_append)
-  using append_eq_append_conv apply auto
-done
-
-lemma list_append_length:
-  assumes "ys \<noteq> []"
-  shows "length xs < length (xs @ ys)"
-  using assms by simp
-
-lemma list_set_memb:
-  assumes "x \<in> set xs"
-  shows "\<exists>ys zs. xs = ys @ [x] @ zs"
-using assms by(induction xs rule: rev_induct, simp, case_tac "x=xa", force+)
+  by(auto simp add: List.map_filter_def)
 
 end
